tests/micro-benchmarks/Unit1.Basic.fst
@@ -359,8 +359,8 @@ assume type bind_test_p :Type0
 assume val lemma_bind_test_p (_:unit) :Tot (squash bind_test_p)
 
 let bind_test1 () :Lemma bind_test_p = lemma_bind_test_p ()
-let bind_test2 () :Lemma bind_test_p = let unfold _ = lemma_bind_test_p () in ()
-let bind_test3 () :Lemma bind_test_p = let unfold x = lemma_bind_test_p () in x
+let bind_test2 () :Lemma bind_test_p = let _ = lemma_bind_test_p () in ()
+let bind_test3 () :Lemma bind_test_p = let x = lemma_bind_test_p () in x
 let bind_test4 () :Lemma bind_test_p = let _ = lemma_bind_test_p () in assert bind_test_p
        
 (* Some tests for the b2t coercion *)
